LambdaS5/coq/LjsRulesCorrectSpecFuns.v
@@ -860,6 +860,7 @@ Definition mutability_of_bools b1 b2 :=
     if b1 then J.mutability_of_bool b2 else J.mutability_immutable.
 
 (* TODO move *)
+(*
 Lemma js_env_record_write_decl_env_lemma : forall jst jeptr s jmut jv jder,
     binds jst jeptr (J.env_record_decl jder) ->
     J.env_record_write_decl_env jst jeptr s jmut jv = 
@@ -872,6 +873,7 @@ Proof.
     erewrite read_binds_inv by eauto.
     reflexivity.
 Qed.
+*)
 
 Lemma decl_env_record_related_write_preserved : forall BR jder obj s jv v b1 b2,
     b1 || !b2 ->
@@ -1046,7 +1048,7 @@ Lemma decl_env_add_binding_lemma : forall BR k jst jc c st st' r jder jeptr ptr 
         (L.attributes_data_intro v b1 true b2))) /\
     r = L.res_value L.value_undefined /\
     ~index (L.object_properties obj) s /\ ~index jder s /\
-    state_invariant BR (J.env_record_write_decl_env jst jeptr s (mutability_of_bools b1 b2) jv) st'.
+    state_invariant BR (J.env_record_write_decl_env jst jeptr jder s (mutability_of_bools b1 b2) jv) st'.
 Proof.
     introv Hlred Hboolcond Hbinds Hjbinds Hcinv Hinv Herel Hvrel Hfact.
     inverts red_exprh Hlred.
@@ -1061,7 +1063,6 @@ Proof.
     }
     {
     destruct obj.
-    erewrite js_env_record_write_decl_env_lemma by eauto.
     eapply state_invariant_modify_env_record_preserved; try eassumption.
     eapply env_record_related_decl.
     lets Hx : decl_env_record_related_write_preserved Hboolcond Hvrel Herel. 
@@ -1084,7 +1085,7 @@ Lemma decl_env_add_mutable_binding_lemma : forall BR k jst jc c st st' r jder je
         (L.attributes_data_intro v true true b2))) /\
     r = L.res_value L.value_undefined /\
     ~index (L.object_properties obj) s /\ ~index jder s /\
-    state_invariant BR (J.env_record_write_decl_env jst jeptr s (J.mutability_of_bool b2) jv) st'.
+    state_invariant BR (J.env_record_write_decl_env jst jeptr jder s (J.mutability_of_bool b2) jv) st'.
 Proof.
     intros. eapply decl_env_add_binding_lemma; eauto.
 Qed.
@@ -1093,7 +1094,7 @@ Lemma create_mutable_binding_some_lemma : forall jst jc jeptr s b2 jder,
     binds jst jeptr (J.env_record_decl jder) ->
     ~index jder s ->
     J.red_expr jst jc (J.spec_env_record_create_mutable_binding jeptr s (Some b2)) 
-        (J.out_void (J.env_record_write_decl_env jst jeptr s (J.mutability_of_bool b2) 
+        (J.out_void (J.env_record_write_decl_env jst jeptr jder s (J.mutability_of_bool b2) 
         (J.value_prim J.prim_undef))).
 Proof.
     introv Hbinds Hnind. eauto_js.
@@ -1103,7 +1104,7 @@ Lemma create_mutable_binding_none_lemma : forall jst jc jeptr s jder,
     binds jst jeptr (J.env_record_decl jder) ->
     ~index jder s ->
     J.red_expr jst jc (J.spec_env_record_create_mutable_binding jeptr s None) 
-        (J.out_void (J.env_record_write_decl_env jst jeptr s (J.mutability_of_bool false) 
+        (J.out_void (J.env_record_write_decl_env jst jeptr jder s (J.mutability_of_bool false) 
         (J.value_prim J.prim_undef))).
 Proof.
     introv Hbinds Hnind. eauto_js.
@@ -1129,20 +1130,17 @@ Lemma create_set_mutable_binding_some_lemma : forall jst jc jeptr s b2 jder jv b
     binds jst jeptr (J.env_record_decl jder) ->
     ~index jder s ->
     J.red_expr jst jc (J.spec_env_record_create_set_mutable_binding jeptr s (Some b2) jv b) 
-        (J.out_void (J.env_record_write_decl_env jst jeptr s (J.mutability_of_bool b2) jv)).
+        (J.out_void (J.env_record_write_decl_env jst jeptr jder s (J.mutability_of_bool b2) jv)).
 Proof.
     introv Hbinds Hnind.
-    erewrite js_env_record_write_decl_env_lemma by eauto.
     eapply J.red_spec_env_record_create_set_mutable_binding.
     eauto_js.
-    erewrite js_env_record_write_decl_env_lemma by eauto.
+    unfolds J.env_record_write_decl_env.
     eapply J.red_spec_env_record_create_set_mutable_binding_1.
-    eapply J.red_spec_env_record_set_mutable_binding.
-    eauto_js.
-    eapply J.red_spec_env_record_set_mutable_binding_1_decl.
-    eauto_js. eauto_js.
-    autorewrite with js_ljs. sets_eq_let x. 
-    erewrite js_env_record_write_decl_env_lemma in EQx by eauto_js.
+    eapply J.red_spec_env_record_set_mutable_binding. eauto_js.
+    eapply J.red_spec_env_record_set_mutable_binding_1_decl. eauto_js. eauto_js.
+    autorewrite with js_ljs. sets_eq_let x.
+    unfolds J.env_record_write_decl_env.
     rew_heap_to_libbag in EQx.
     rew_bag_simpl in EQx.
     substs. eauto_js.
@@ -1154,23 +1152,22 @@ Lemma create_set_mutable_binding_none_lemma : forall jst jc jeptr s jder jv b,
     binds jst jeptr (J.env_record_decl jder) ->
     ~index jder s ->
     J.red_expr jst jc (J.spec_env_record_create_set_mutable_binding jeptr s None jv b) 
-        (J.out_void (J.env_record_write_decl_env jst jeptr s (J.mutability_of_bool false) jv)).
+        (J.out_void (J.env_record_write_decl_env jst jeptr jder s (J.mutability_of_bool false) jv)).
 Proof.
     introv Hbinds Hnind.
-    erewrite js_env_record_write_decl_env_lemma by eauto.
     eapply J.red_spec_env_record_create_set_mutable_binding.
     eauto_js.
-    erewrite js_env_record_write_decl_env_lemma by eauto.
+    unfolds J.env_record_write_decl_env.
     eapply J.red_spec_env_record_create_set_mutable_binding_1.
     eapply J.red_spec_env_record_set_mutable_binding.
     rew_heap_to_libbag. eauto_js.
     eapply J.red_spec_env_record_set_mutable_binding_1_decl.
     rew_heap_to_libbag. eauto_js. eauto_js.
-    autorewrite with js_ljs. sets_eq_let x. 
-    erewrite js_env_record_write_decl_env_lemma in EQx by eauto_js.
-    rew_heap_to_libbag in EQx.
+    autorewrite with js_ljs. sets_eq_let x.
+    unfolds J.env_record_write_decl_env.
+    repeat rew_heap_to_libbag in EQx.
     rew_bag_simpl in EQx.
     substs. eauto_js.
-Qed. 
+Qed.
 
 Hint Resolve create_set_mutable_binding_none_lemma : js_ljs.
